clean up, define common [no_wipe] and [no_crash] helpers for the crash_effect relation

src/Refinement/Interface.v
@@ -49,6 +49,12 @@ Definition post_step {opT State}
     exists state', step op state v state' /\
           bg_step state' state''.
 
+Definition no_wipe State (state state' : State) : Prop := state' = state.
+Hint Unfold no_wipe.
+
+Definition no_crash State (state state' : State) : Prop := False.
+Hint Unfold no_crash.
+
 (* The specification for each operation. Note that after recovery, the abstract
 state is expected to be atomic. *)
 Definition op_spec_wipe opT `(api: InterfaceAPI opT State) `(op: opT T) : Specification unit T unit State :=
