src/Variables/VariablesImpl.v
@@ -15,7 +15,7 @@ Module Vars <: VarsAPI.
 
   Axiom read_ok : forall v, prog_spec (read_spec v) (read v) recover abstr.
   Axiom write_ok : forall v val, prog_spec (write_spec v val) (write v val) recover abstr.
-  Axiom recover_noop : rec_noop recover abstr wipe.
+  Axiom recover_noop : rec_noop recover abstr (@no_crash _).
 
 End Vars.
 
